iris_derived_rules.v
@@ -1,0 +1,37 @@
+Require Import ssreflect.
+Require Import world_prop core_lang lang masks iris_core iris_plog iris_vs_rules iris_ht_rules.
+Require Import ModuRes.RA ModuRes.UPred ModuRes.BI ModuRes.PreoMet ModuRes.Finmap.
+
+Set Bullet Behavior "Strict Subproofs".
+
+Module Type IRIS_DERIVED_RULES (RL : RA_T) (C : CORE_LANG) (R: IRIS_RES RL C) (WP: WORLD_PROP R) (CORE: IRIS_CORE RL C R WP) (PLOG: IRIS_PLOG RL C R WP CORE) (VS_RULES: IRIS_VS_RULES RL C R WP CORE PLOG) (HT_RULES: IRIS_HT_RULES RL C R WP CORE PLOG).
+  Export VS_RULES.
+  Export HT_RULES.
+
+  Local Open Scope lang_scope.
+  Local Open Scope ra_scope.
+  Local Open Scope bi_scope.
+  Local Open Scope iris_scope.
+
+  Section DerivedRules.
+
+    Existing Instance LP_isval.
+
+    Implicit Types (P : Props) (i : nat) (m : mask) (e : expr) (r : res).
+
+    Lemma vsFalse m1 m2 :
+      valid (vs m1 m2 ⊥ ⊥).
+    Proof.
+      rewrite ->valid_iff, box_top.
+      unfold vs; apply box_intro.
+      rewrite <- and_impl, and_projR.
+      apply bot_false.
+    Qed.
+
+  End DerivedRules. 
+
+End IRIS_DERIVED_RULES.
+
+Module IrisDerivedRules (RL : RA_T) (C : CORE_LANG) (R: IRIS_RES RL C) (WP: WORLD_PROP R) (CORE: IRIS_CORE RL C R WP) (PLOG: IRIS_PLOG RL C R WP CORE) (VS_RULES: IRIS_VS_RULES RL C R WP CORE PLOG) (HT_RULES: IRIS_HT_RULES RL C R WP CORE PLOG) : IRIS_DERIVED_RULES RL C R WP CORE PLOG VS_RULES HT_RULES.
+  Include IRIS_DERIVED_RULES RL C R WP CORE PLOG VS_RULES HT_RULES.
+End IrisDerivedRules.
